Return error message

proof_checker.v
@@ -219,39 +219,63 @@ Fixpoint ends_with_assert(s: stmt)(P: term): bool :=
   | _ => false
   end.
 
-Fixpoint is_valid_proof_outline(s: stmt): bool :=
+Inductive result(A E: Type) :=
+  ok(a: A)
+| error(e: E)
+.
+Arguments ok {A E} _.
+Arguments error {A E} _.
+
+Fixpoint check_proof_outline(s: stmt): result unit (loc * string) :=
   match s with
     Assert laP P _ ;; (Assert laP' P' (Some j) ;; _) as s =>
-    is_valid_entailment P P' j && is_valid_proof_outline s
+    if is_valid_entailment P P' j then
+      check_proof_outline s
+    else
+      error (laP', "Could not verify entailment")
   | Assert laP P _ ;; Assign lass x t ;; (Assert laQ Q _ ;; _) as s =>
-    term_equivb P (subst x t Q) && is_valid_proof_outline s
+    if term_equivb P (subst x t Q) then
+      check_proof_outline s
+    else
+      error (laP, "Assignment precondition does not match postcondition with RHS substituted for LHS")
   | Assert laInv Inv _ ;; (While lw C ((Assert laP P _ ;; _) as body)) ;; ((Assert laQ Q _ ;; _) as s) =>
-    term_equivb P (BinOp laInv And Inv C) && ends_with_assert body Inv &&
-    is_valid_proof_outline body && term_equivb Q (BinOp laInv And Inv (Not laInv C)) &&
-    is_valid_proof_outline s
-  | Assert laP P _ ;; Pass lp => true
-  | _ => false
+    if term_equivb P (BinOp laInv And Inv C) then
+      if ends_with_assert body Inv then
+        match check_proof_outline body with
+          ok _ =>
+          if term_equivb Q (BinOp laInv And Inv (Not laInv C)) then
+            check_proof_outline s
+          else
+            error (laQ, "Loop postcondition does not match conjunction of invariant and negation of condition")
+        | error e => error e
+        end
+      else
+        error (lw, "Body of loop does not end with an assert statement that asserts the loop invariant")
+    else
+      error (laP, "Loop body precondition does not match conjunction of invariant and condition")
+  | Assert laP P _ ;; Pass lp => ok tt
+  | _ => error (loc_of_stmt s, "Malformed proof outline")
   end.
 
-Goal is_valid_proof_outline (
+Goal check_proof_outline (
   Assert (locN 0) (BinOp (locN 1) Eq (Var (locN 2) "x") (Val (locN 3) 1)) None;;
   Assert (locN 4) (BinOp (locN 5) Eq (Var (locN 6) "x") (Val (locN 7) 1)) (Some (JZ (locN 8)));;
   Pass (locN 9)
-) = true.
+) = ok tt.
 Proof.
   reflexivity.
 Qed.
 
-Goal is_valid_proof_outline (
+Goal check_proof_outline (
   Assert (locN 0) (BinOp (locN 1) And (BinOp (locN 2) Eq (Var (locN 3) "x") (Val (locN 4) 1)) (BinOp (locN 5) Eq (Var (locN 6) "y") (Val (locN 7) 1))) None;;
   Assert (locN 8) (BinOp (locN 9) And (BinOp (locN 10) Eq (Var (locN 11) "y") (Val (locN 12) 1)) (BinOp (locN 13) Eq (Var (locN 14) "x") (Val (locN 15) 1))) (Some (JZ (locN 16)));;
   Pass (locN 17)
-) = true.
+) = ok tt.
 Proof.
   reflexivity.
 Qed.
 
-Goal is_valid_proof_outline (
+Goal check_proof_outline (
     Assert (locN 0) (BinOp (locN 1) And (BinOp (locN 2) Eq (Var (locN 14) "r") (BinOp (locN 3) Sub (Var (locN 4) "n") (Var (locN 5) "i"))) (Not (locN 6) (BinOp (locN 7) Eq (Var (locN 8) "i") (Val (locN 9) 0)))) None;;
     Assert (locN 10) (BinOp (locN 11) Eq (BinOp (locN 12) Add (Var (locN 13) "r") (Val (locN 15) 1)) (BinOp (locN 16) Sub (Var (locN 17) "n") (BinOp (locN 18) Sub (Var (locN 19) "i") (Val (locN 20) 1)))) (Some (JZ_at (locN 21) (locN 22) 0));;
     Assign (locN 23) "i" (BinOp (locN 24) Sub (Var (locN 25) "i") (Val (locN 26) 1));;
@@ -259,7 +283,7 @@ Goal is_valid_proof_outline (
     Assign (locN 35) "r" (BinOp (locN 36) Add (Var (locN 37) "r") (Val (locN 38) 1));;
     Assert (locN 39) (BinOp (locN 40) Eq (Var (locN 41) "r") (BinOp (locN 42) Sub (Var (locN 43) "n") (Var (locN 44) "i"))) None;;
     Pass (locN 45)
-) = true.
+) = ok tt.
 Proof.
   reflexivity.
 Qed.
@@ -279,7 +303,7 @@ Proof.
 Qed.
 *)
 
-Goal is_valid_proof_outline outline1 = true.
+Goal check_proof_outline outline1 = ok tt.
 Proof.
   reflexivity.
 Qed.
